Valaig/Sat/Std.lean
@@ -26,6 +26,9 @@ private def walker (aig : WFAig) (reset : Bool) : aig.CachingForwardsWalker (Std
   cacheMotive std size le sm var lt lit :=
     lit.var.idx < std.decls.size
 
+  init := .empty
+  initState := by grind
+
   step var std cache valid size sm cm :=
     let map (lit : Lit) (valid : lit.var < var := by grind) :=
       cache.mapLit lit |>.toRef std
@@ -52,11 +55,10 @@ private def walker (aig : WFAig) (reset : Bool) : aig.CachingForwardsWalker (Std
 end toStd
 
 def toStd (aig : WFAig) (reset : Bool) : (aig' : Std.Sat.AIG LeafIdx) × (Lit.In aig -> aig'.Ref) :=
-  let res := (toStd.walker aig reset).walk Std.Sat.AIG.empty (by grind [toStd.walker])
-  ⟨res.fst, fun lit => (res.snd.mapLit lit.val).toRef res.fst <|
-    by
-      have := CachingForwardsWalker.cacheMotive_walk (walker := toStd.walker aig reset) Std.Sat.AIG.empty (by grind [toStd.walker])
-      grind [toStd.walker]
-  ⟩
+  let walker := toStd.walker aig reset
+  let res := walker.walk
+
+  have := walker.cacheMotive_walk
+  ⟨res.fst, fun lit => (res.snd.mapLit lit.val).toRef res.fst (by grind [toStd.walker])⟩
 
 end Valaig.Sat
